20) Замена переменной – общий случай.\\
$ T= \sum\limits_{\substack{i'_1,\dots,i'_q \in \ovl{1,n}\\ j'_1,\dots,j'_p \in \ovl{1,n}}} T_{j'_1,\dots,j'_p}^{i'_1,\dots,i'_q} e^{j'_1,\dots,j'_p}_{i'_1,\dots,i'_q}$. $e_i=\sum\limits_{j=1}^nC_{ji}\hat{e}_j$ и $e^i=\sum D_{ji}\hat{e}^j$. Раскрыть скобки, поменять суммирование. Должно получиться $\hat{T}_{j_1,\dots,j_p}^{i_1,\dots,i_q}=\sum\limits_{\substack{i'_1,\dots,i'_q \in \ovl{1,n}\\ j'_1,\dots,j'_p \in \ovl{1,n}}} \,\,\prod\limits_{t\in \ovl{1,p}} D_{j_t,j'_t} \prod\limits_{s\in \ovl{1,q}} C_{i_s,i'_s}  \,\,T_{j'_1,\dots,j'_p}^{i'_1,\dots,i'_q}.$